@@ -1,0 +1,10 @@
+/-
+`sys_dup` meets its specification, given `argfd`, `fdalloc` and `filedup`.
+-/
+import Xv6.ProofSysDup
+
+namespace Xv6
+
+theorem SysDup (AF : ARGFD) (FD : FDALLOC) (FU : FILEDUP) : SYSDUP := sys_dup_proof AF FD FU
+
+end Xv6
